LaTeX code is now generated directly from theory file.

doc-src/TutorialI/Inductive/Advanced.thy
@@ -1,10 +1,61 @@
 (* ID:         $Id$ *)
-theory Advanced imports Even begin
+(*<*)theory Advanced imports Even uses "../../antiquote_setup.ML" begin(*>*)
 
+text {*
+The premises of introduction rules may contain universal quantifiers and
+monotone functions.  A universal quantifier lets the rule 
+refer to any number of instances of 
+the inductively defined set.  A monotone function lets the rule refer
+to existing constructions (such as ``list of'') over the inductively defined
+set.  The examples below show how to use the additional expressiveness
+and how to reason from the resulting definitions.
+*}
+
+subsection{* Universal Quantifiers in Introduction Rules \label{sec:gterm-datatype} *}
+
+text {*
+\index{ground terms example|(}%
+\index{quantifiers!and inductive definitions|(}%
+As a running example, this section develops the theory of \textbf{ground
+terms}: terms constructed from constant and function 
+symbols but not variables. To simplify matters further, we regard a
+constant as a function applied to the null argument  list.  Let us declare a
+datatype @{text gterm} for the type of ground  terms. It is a type constructor
+whose argument is a type of  function symbols. 
+*}
 
 datatype 'f gterm = Apply 'f "'f gterm list"
 
-datatype integer_op = Number int | UnaryMinus | Plus;
+text {*
+To try it out, we declare a datatype of some integer operations: 
+integer constants, the unary minus operator and the addition 
+operator.
+*}
+
+datatype integer_op = Number int | UnaryMinus | Plus
+
+text {*
+Now the type @{typ "integer_op gterm"} denotes the ground 
+terms built over those symbols.
+
+The type constructor @{text gterm} can be generalized to a function 
+over sets.  It returns 
+the set of ground terms that can be formed over a set @{text F} of function symbols. For
+example,  we could consider the set of ground terms formed from the finite 
+set @{text "{Number 2, UnaryMinus, Plus}"}.
+
+This concept is inductive. If we have a list @{text args} of ground terms 
+over~@{text F} and a function symbol @{text f} in @{text F}, then we 
+can apply @{text f} to @{text args} to obtain another ground term. 
+The only difficulty is that the argument list may be of any length. Hitherto, 
+each rule in an inductive definition referred to the inductively 
+defined set a fixed number of times, typically once or twice. 
+A universal quantifier in the premise of the introduction rule 
+expresses that every element of @{text args} belongs
+to our inductively defined set: is a ground term 
+over~@{text F}.  The function @{term set} denotes the set of elements in a given 
+list. 
+*}
 
 inductive_set
   gterms :: "'f set \<Rightarrow> 'f gterm set"
@@ -13,76 +64,55 @@ where
 step[intro!]: "\<lbrakk>\<forall>t \<in> set args. t \<in> gterms F;  f \<in> F\<rbrakk>
                \<Longrightarrow> (Apply f args) \<in> gterms F"
 
+text {*
+To demonstrate a proof from this definition, let us 
+show that the function @{term gterms}
+is \textbf{monotone}.  We shall need this concept shortly.
+*}
+
 lemma gterms_mono: "F\<subseteq>G \<Longrightarrow> gterms F \<subseteq> gterms G"
 apply clarify
 apply (erule gterms.induct)
-txt{*
-@{subgoals[display,indent=0,margin=65]}
-*};
 apply blast
 done
-
-
-text{*
-@{thm[display] even.cases[no_vars]}
-\rulename{even.cases}
-
-Just as a demo I include
-the two forms that Markus has made available. First the one for binding the
-result to a name 
-
-*}
-
-inductive_cases Suc_Suc_cases [elim!]:
-  "Suc(Suc n) \<in> even"
-
-thm Suc_Suc_cases;
-
-text{*
-@{thm[display] Suc_Suc_cases[no_vars]}
-\rulename{Suc_Suc_cases}
-
-and now the one for local usage:
-*}
-
-lemma "Suc(Suc n) \<in> even \<Longrightarrow> P n";
-apply (ind_cases "Suc(Suc n) \<in> even");
-oops
-
-inductive_cases gterm_Apply_elim [elim!]: "Apply f args \<in> gterms F"
-
-text{*this is what we get:
-
-@{thm[display] gterm_Apply_elim[no_vars]}
-\rulename{gterm_Apply_elim}
-*}
-
-lemma gterms_IntI [rule_format, intro!]:
-     "t \<in> gterms F \<Longrightarrow> t \<in> gterms G \<longrightarrow> t \<in> gterms (F\<inter>G)"
+(*<*)
+lemma gterms_mono: "F\<subseteq>G \<Longrightarrow> gterms F \<subseteq> gterms G"
+apply clarify
 apply (erule gterms.induct)
+(*>*)
 txt{*
-@{subgoals[display,indent=0,margin=65]}
-*};
-apply blast
-done
-
-
-text{*
-@{thm[display] mono_Int[no_vars]}
-\rulename{mono_Int}
+Intuitively, this theorem says that
+enlarging the set of function symbols enlarges the set of ground 
+terms. The proof is a trivial rule induction.
+First we use the @{text clarify} method to assume the existence of an element of
+@{term "gterms F"}.  (We could have used @{text "intro subsetI"}.)  We then
+apply rule induction. Here is the resulting subgoal:
+@{subgoals[display,indent=0]}
+The assumptions state that @{text f} belongs 
+to~@{text F}, which is included in~@{text G}, and that every element of the list @{text args} is
+a ground term over~@{text G}.  The @{text blast} method finds this chain of reasoning easily.  
 *}
+(*<*)oops(*>*)
+text {*
+\begin{warn}
+Why do we call this function @{text gterms} instead 
+of @{text gterm}?  A constant may have the same name as a type.  However,
+name  clashes could arise in the theorems that Isabelle generates. 
+Our choice of names keeps @{text gterms.induct} separate from 
+@{text gterm.induct}.
+\end{warn}
 
-lemma gterms_Int_eq [simp]:
-     "gterms (F\<inter>G) = gterms F \<inter> gterms G"
-by (blast intro!: mono_Int monoI gterms_mono)
-
-
-text{*the following declaration isn't actually used*}
-consts integer_arity :: "integer_op \<Rightarrow> nat"
-primrec
-"integer_arity (Number n)        = 0"
-"integer_arity UnaryMinus        = 1"
-"integer_arity Plus              = 2"
+Call a term \textbf{well-formed} if each symbol occurring in it is applied
+to the correct number of arguments.  (This number is called the symbol's
+\textbf{arity}.)  We can express well-formedness by
+generalizing the inductive definition of
+\isa{gterms}.
+Suppose we are given a function called @{text arity}, specifying the arities
+of all symbols.  In the inductive step, we have a list @{text args} of such
+terms and a function  symbol~@{text f}. If the length of the list matches the
+function's arity  then applying @{text f} to @{text args} yields a well-formed
+term.
+*}
 
 inductive_set
   well_formed_gterm :: "('f \<Rightarrow> nat) \<Rightarrow> 'f gterm set"
@@ -92,6 +122,32 @@ step[intro!]: "\<lbrakk>\<forall>t \<in> set args. t \<in> well_formed_gterm ari
                 length args = arity f\<rbrakk>
                \<Longrightarrow> (Apply f args) \<in> well_formed_gterm arity"
 
+text {*
+The inductive definition neatly captures the reasoning above.
+The universal quantification over the
+@{text set} of arguments expresses that all of them are well-formed.%
+\index{quantifiers!and inductive definitions|)}
+*}
+
+subsection{* Alternative Definition Using a Monotone Function *}
+
+text {*
+\index{monotone functions!and inductive definitions|(}% 
+An inductive definition may refer to the
+inductively defined  set through an arbitrary monotone function.  To
+demonstrate this powerful feature, let us
+change the  inductive definition above, replacing the
+quantifier by a use of the function @{term lists}. This
+function, from the Isabelle theory of lists, is analogous to the
+function @{term gterms} declared above: if @{text A} is a set then
+@{term "lists A"} is the set of lists whose elements belong to
+@{term A}.  
+
+In the inductive definition of well-formed terms, examine the one
+introduction rule.  The first premise states that @{text args} belongs to
+the @{text lists} of well-formed terms.  This formulation is more
+direct, if more obscure, than using a universal quantifier.
+*}
 
 inductive_set
   well_formed_gterm' :: "('f \<Rightarrow> nat) \<Rightarrow> 'f gterm set"
@@ -102,40 +158,213 @@ step[intro!]: "\<lbrakk>args \<in> lists (well_formed_gterm' arity);
                \<Longrightarrow> (Apply f args) \<in> well_formed_gterm' arity"
 monos lists_mono
 
+text {*
+We cite the theorem @{text lists_mono} to justify 
+using the function @{term lists}.%
+\footnote{This particular theorem is installed by default already, but we
+include the \isakeyword{monos} declaration in order to illustrate its syntax.}
+@{named_thms [display,indent=0] lists_mono [no_vars] (lists_mono)}
+Why must the function be monotone?  An inductive definition describes
+an iterative construction: each element of the set is constructed by a
+finite number of introduction rule applications.  For example, the
+elements of \isa{even} are constructed by finitely many applications of
+the rules
+@{thm [display,indent=0] even.intros [no_vars]}
+All references to a set in its
+inductive definition must be positive.  Applications of an
+introduction rule cannot invalidate previous applications, allowing the
+construction process to converge.
+The following pair of rules do not constitute an inductive definition:
+\begin{trivlist}
+\item @{term "0 \<in> even"}
+\item @{term "n \<notin> even \<Longrightarrow> (Suc n) \<in> even"}
+\end{trivlist}
+Showing that 4 is even using these rules requires showing that 3 is not
+even.  It is far from trivial to show that this set of rules
+characterizes the even numbers.  
+
+Even with its use of the function \isa{lists}, the premise of our
+introduction rule is positive:
+@{thm_style [display,indent=0] prem1 step [no_vars]}
+To apply the rule we construct a list @{term args} of previously
+constructed well-formed terms.  We obtain a
+new term, @{term "Apply f args"}.  Because @{term lists} is monotone,
+applications of the rule remain valid as new terms are constructed.
+Further lists of well-formed
+terms become available and none are taken away.%
+\index{monotone functions!and inductive definitions|)} 
+*}
+
+subsection{* A Proof of Equivalence *}
+
+text {*
+We naturally hope that these two inductive definitions of ``well-formed'' 
+coincide.  The equality can be proved by separate inclusions in 
+each direction.  Each is a trivial rule induction. 
+*}
+
 lemma "well_formed_gterm arity \<subseteq> well_formed_gterm' arity"
 apply clarify
-txt{*
-The situation after clarify
-@{subgoals[display,indent=0,margin=65]}
-*};
 apply (erule well_formed_gterm.induct)
-txt{*
-note the induction hypothesis!
-@{subgoals[display,indent=0,margin=65]}
-*};
 apply auto
 done
-
-
-
+(*<*)
+lemma "well_formed_gterm arity \<subseteq> well_formed_gterm' arity"
+apply clarify
+apply (erule well_formed_gterm.induct)
+(*>*)
+txt {*
+The @{text clarify} method gives
+us an element of @{term "well_formed_gterm arity"} on which to perform 
+induction.  The resulting subgoal can be proved automatically:
+@{subgoals[display,indent=0]}
+This proof resembles the one given in
+{\S}\ref{sec:gterm-datatype} above, especially in the form of the
+induction hypothesis.  Next, we consider the opposite inclusion:
+*}
+(*<*)oops(*>*)
 lemma "well_formed_gterm' arity \<subseteq> well_formed_gterm arity"
 apply clarify
-txt{*
-The situation after clarify
-@{subgoals[display,indent=0,margin=65]}
-*};
 apply (erule well_formed_gterm'.induct)
-txt{*
-note the induction hypothesis!
-@{subgoals[display,indent=0,margin=65]}
-*};
 apply auto
 done
+(*<*)
+lemma "well_formed_gterm' arity \<subseteq> well_formed_gterm arity"
+apply clarify
+apply (erule well_formed_gterm'.induct)
+(*>*)
+txt {*
+The proof script is identical, but the subgoal after applying induction may
+be surprising:
+@{subgoals[display,indent=0,margin=65]}
+The induction hypothesis contains an application of @{term lists}.  Using a
+monotone function in the inductive definition always has this effect.  The
+subgoal may look uninviting, but fortunately 
+@{term lists} distributes over intersection:
+@{named_thms [display,indent=0] lists_Int_eq [no_vars] (lists_Int_eq)}
+Thanks to this default simplification rule, the induction hypothesis 
+is quickly replaced by its two parts:
+\begin{trivlist}
+\item @{term "args \<in> lists (well_formed_gterm' arity)"}
+\item @{term "args \<in> lists (well_formed_gterm arity)"}
+\end{trivlist}
+Invoking the rule @{text well_formed_gterm.step} completes the proof.  The
+call to @{text auto} does all this work.
 
-
-text{*
-@{thm[display] lists_Int_eq[no_vars]}
+This example is typical of how monotone functions
+\index{monotone functions} can be used.  In particular, many of them
+distribute over intersection.  Monotonicity implies one direction of
+this set equality; we have this theorem:
+@{named_thms [display,indent=0] mono_Int [no_vars] (mono_Int)}
 *}
+(*<*)oops(*>*)
+
+
+subsection{* Another Example of Rule Inversion *}
+
+text {*
+\index{rule inversion|(}%
+Does @{term gterms} distribute over intersection?  We have proved that this
+function is monotone, so @{text mono_Int} gives one of the inclusions.  The
+opposite inclusion asserts that if @{term t} is a ground term over both of the
+sets
+@{term F} and~@{term G} then it is also a ground term over their intersection,
+@{term "F \<inter> G"}.
+*}
+
+lemma gterms_IntI:
+     "t \<in> gterms F \<Longrightarrow> t \<in> gterms G \<longrightarrow> t \<in> gterms (F\<inter>G)"
+(*<*)oops(*>*)
+text {*
+Attempting this proof, we get the assumption 
+@{term "Apply f args \<in> gterms G"}, which cannot be broken down. 
+It looks like a job for rule inversion:\cmmdx{inductive\protect\_cases}
+*}
+
+inductive_cases gterm_Apply_elim [elim!]: "Apply f args \<in> gterms F"
+
+text {*
+Here is the result.
+@{named_thms [display,indent=0,margin=50] gterm_Apply_elim [no_vars] (gterm_Apply_elim)}
+This rule replaces an assumption about @{term "Apply f args"} by 
+assumptions about @{term f} and~@{term args}.  
+No cases are discarded (there was only one to begin
+with) but the rule applies specifically to the pattern @{term "Apply f args"}.
+It can be applied repeatedly as an elimination rule without looping, so we
+have given the @{text "elim!"} attribute. 
+
+Now we can prove the other half of that distributive law.
+*}
+
+lemma gterms_IntI [rule_format, intro!]:
+     "t \<in> gterms F \<Longrightarrow> t \<in> gterms G \<longrightarrow> t \<in> gterms (F\<inter>G)"
+apply (erule gterms.induct)
+apply blast
+done
+(*<*)
+lemma "t \<in> gterms F \<Longrightarrow> t \<in> gterms G \<longrightarrow> t \<in> gterms (F\<inter>G)"
+apply (erule gterms.induct)
+(*>*)
+txt {*
+The proof begins with rule induction over the definition of
+@{term gterms}, which leaves a single subgoal:  
+@{subgoals[display,indent=0,margin=65]}
+To prove this, we assume @{term "Apply f args \<in> gterms G"}.  Rule inversion,
+in the form of @{text gterm_Apply_elim}, infers
+that every element of @{term args} belongs to 
+@{term "gterms G"}; hence (by the induction hypothesis) it belongs
+to @{term "gterms (F \<inter> G)"}.  Rule inversion also yields
+@{term "f \<in> G"} and hence @{term "f \<in> F \<inter> G"}. 
+All of this reasoning is done by @{text blast}.
+
+\smallskip
+Our distributive law is a trivial consequence of previously-proved results:
+*}
+(*<*)oops(*>*)
+lemma gterms_Int_eq [simp]:
+     "gterms (F \<inter> G) = gterms F \<inter> gterms G"
+by (blast intro!: mono_Int monoI gterms_mono)
+
+text_raw {*
+\index{rule inversion|)}%
+\index{ground terms example|)}
+
+
+\begin{isamarkuptext}
+\begin{exercise}
+A function mapping function symbols to their 
+types is called a \textbf{signature}.  Given a type 
+ranging over type symbols, we can represent a function's type by a
+list of argument types paired with the result type. 
+Complete this inductive definition:
+\begin{isabelle}
+*}
+
+inductive_set
+  well_typed_gterm :: "('f \<Rightarrow> 't list * 't) \<Rightarrow> ('f gterm * 't)set"
+  for sig :: "'f \<Rightarrow> 't list * 't"
+(*<*)
+where
+step[intro!]: 
+    "\<lbrakk>\<forall>pair \<in> set args. pair \<in> well_typed_gterm sig; 
+      sig f = (map snd args, rtype)\<rbrakk>
+     \<Longrightarrow> (Apply f (map fst args), rtype) 
+         \<in> well_typed_gterm sig"
+(*>*)
+text_raw {*
+\end{isabelle}
+\end{exercise}
+\end{isamarkuptext}
+*}
+
+(*<*)
+
+text{*the following declaration isn't actually used*}
+consts integer_arity :: "integer_op \<Rightarrow> nat"
+primrec
+"integer_arity (Number n)        = 0"
+"integer_arity UnaryMinus        = 1"
+"integer_arity Plus              = 2"
 
 text{* the rest isn't used: too complicated.  OK for an exercise though.*}
 
@@ -145,17 +374,6 @@ where
   Number:     "(Number n,   ([], ())) \<in> integer_signature"
 | UnaryMinus: "(UnaryMinus, ([()], ())) \<in> integer_signature"
 | Plus:       "(Plus,       ([(),()], ())) \<in> integer_signature"
-
-
-inductive_set
-  well_typed_gterm :: "('f \<Rightarrow> 't list * 't) \<Rightarrow> ('f gterm * 't)set"
-  for sig :: "'f \<Rightarrow> 't list * 't"
-where
-step[intro!]: 
-    "\<lbrakk>\<forall>pair \<in> set args. pair \<in> well_typed_gterm sig; 
-      sig f = (map snd args, rtype)\<rbrakk>
-     \<Longrightarrow> (Apply f (map fst args), rtype) 
-         \<in> well_typed_gterm sig"
 
 inductive_set
   well_typed_gterm' :: "('f \<Rightarrow> 't list * 't) \<Rightarrow> ('f gterm * 't)set"
@@ -183,4 +401,4 @@ done
 
 
 end
-
+(*>*)
